implement and prove splitting (no root node, no intervals)

src/Insert.v
@@ -6,36 +6,61 @@ Require Import NaryTree.
 Require Import BPlusTree.
 
 Section nary_tree.
+  Context (b : nat).
 
-  Fixpoint Insert_list (target : Z) (l : list Z) : list Z :=
+  Fixpoint insert_list_spec (target : Z) (l : list Z) : list Z :=
     match l with
     | [] => [target]
     | x :: xs => if Z.eqb x target
                then x :: xs
                else if Z.ltb x target
-                    then x :: Insert_list target xs
+                    then x :: insert_list_spec target xs
                     else target :: x :: xs
     end.
 
-  Fixpoint Insert_nary_tree (target : Z) (t : nary_tree) : nary_tree :=
-    match t with
-    | leaf interval vals => leaf interval (Insert_list target vals)
-    | node interval branches =>
-        node interval
-          ((fix insert_aux (l : list nary_tree) :=
-              match l with
-              | [] => [leaf (target, target) [target]]
-              | t :: ts =>
-                  let (low, high) := (match t with leaf interval _ | node interval _ => interval end) in
-                  if andb (Z.leb low target) (Z.leb target high)
-                  then Insert_nary_tree target t :: ts
-                  else t :: insert_aux ts
-              end) branches)
-    end.
+  (* Definition insert_bplus_tree_spec (target : Z) (t : bplus_tree) := *)
+  (*   match t with *)
+  (*   | root_leaf (low, high) vals => *)
+  (*       let new_vals := insert_list_spec target vals in *)
+  (*       if Z.ltb b (length new_vals) *)
+  (*       then *)
+  (*         let left_vals := firstn (b/2) new_vals in *)
+  (*         let right_vals := skipn (b/2) new_vals in *)
+  (*         let left_interval := (low, List.last left_vals high) in *)
+  (*         let right_interval := (hd low right_vals, high) in *)
+  (*         (* TODO: should change interval *) *)
+  (*         root_node (low, high) (leaf left_interval left_vals :: [leaf right_interval right_vals]) *)
+  (*       else *)
+  (*         root_leaf (low, high) new_vals *)
+  (*   | root_node interval branches => *)
+  (*       let new_branches := *)
+  (*         ((fix insert_aux (l : list nary_tree) := *)
+  (*             match l with *)
+  (*             | [] => [] *)
+  (*             | t :: ts => *)
+  (*                 let (low, high) := (match t with leaf interval _ | node interval _ => interval end) in *)
+  (*                 if andb (Z.leb low target) (Z.leb target high) *)
+  (*                 then *)
+  (*                   let (new_t1, new_t2) := insert_nary_tree_spec target t in *)
+  (*                   match new_t2 with *)
+  (*                   | None => new_t1 :: ts *)
+  (*                   | Some new_t2' => new_t1 :: new_t2' :: ts *)
+  (*                   end *)
+  (*                 else t :: insert_aux ts *)
+  (*             end) branches) in *)
+  (*       (* TODO: should change interval *) *)
+  (*       if Z.leb b (length new_branches) *)
+  (*       then *)
+  (*         root_node interval *)
+  (*           ([node interval (firstn (b/2) new_branches)] ++ [node interval (skipn (b/2) new_branches)]) *)
+  (*       else *)
+  (*         root_node interval branches *)
+  (*   end. *)
 End nary_tree.
 
 Section bplus_tree.
   Section bplus_tree_algos.
+    Context (b : nat).
 
     Definition insert_list : val :=
       rec: "insert_list" "arg" :=
@@ -57,48 +82,30 @@ Section bplus_tree.
               else SOME (ref ("target", SOME "l"))
         end.
 
-    Definition insert_bplus_tree : val :=
-      rec: "insert_bplus_tree" "arg" :=
-        let: "t" := Fst "arg" in
-        let: "target" := Snd "arg" in
-        match: "t" with
-          InjL "ptr" =>
-            let: "lhd" := Snd !"ptr" in
-            let: "new" := insert_list ("lhd", "target") in
-            (* should change interval here *)
-            "ptr" <- (Fst !"ptr", "new") ;;
-            "t"
-        | InjR "ptr" =>
-            let: "lhd" := Snd !"ptr" in
-            let: "new" :=
-              (rec: "insert_node_list" "arg" :=
-                 let: "p" := Fst "arg" in
-                 let: "target" := Snd "arg" in
-                 match: "p" with
-                   NONE =>
-                     let: "l" := SOME (ref ("target", NONE)) in
-                     let: "t" := ref (("target", "target"), "l") in
-                     SOME (ref (token_leaf_e "t", NONE))
-                 | SOME "l" =>
-                     let: "thd" := Fst !"l" in
-                     let: "interval" :=
-                       match: "thd" with
-                         InjL "ptr" => Fst !"ptr"
-                       | InjR "ptr" => Fst !"ptr"
-                       end in
-                     let: "low" := Fst "interval" in
-                     let: "high" := Snd "interval" in
-                     (if: (BinOp LeOp "low" "target") && (BinOp LeOp "target" "high")
-                      then let: "newt" := "insert_bplus_tree" ("thd", "target") in
-                           (* should change interval here *)
-                           "l" <- ("newt", Snd !"l")
-                      else let: "newl" := "insert_node_list" (Snd !"l", "target") in
-                           "l" <- ("thd", "newl")) ;;
-                     SOME "l"
-                 end) ("lhd", "target") in
-            "ptr" <- (Fst !"ptr", "new") ;;
-            token_branch_e "ptr"
-        end%E.
+    Definition length_list : val :=
+      rec: "length_list" "p" :=
+        match: "p" with
+          NONE => #0
+        | SOME "l" => #1 + "length_list" (Snd !"l")
+        end.
+
+    Definition split_list : val :=
+      rec: "split_list" "arg" :=
+        let: "p" := Fst "arg" in
+        let: "n" := Snd "arg" in
+        if: "n" = #0
+        then (NONEV, "p")
+        else
+          match: "p" with
+            NONE => (NONEV, NONEV)
+          | SOME "l" =>
+              let: "x" := Fst !"l" in
+              let: "rest" := Snd !"l" in
+              let: "rec" := "split_list" ("rest", "n" - #1) in
+              "l" <- ("x", Fst "rec") ;;
+              (SOME "l", Snd "rec")
+          end.
+
   End bplus_tree_algos.
 
   Section bplus_tree_proofs.
@@ -120,8 +127,8 @@ Section bplus_tree.
       lia.
     Qed.
 
-    Lemma insert_list_spec (v : val) (l : list tval) (target : tval):
-      {{{ is_list v (map (fun (x : tval) => #x) l) }}} insert_list (v, (#target))%V {{{ r, RET r; is_list r (map (fun (x : tval) => #x) (Insert_list target l)) }}}.
+    Lemma insert_list_spec_proof (v : val) (l : list tval) (target : tval):
+      {{{ is_list v (map (fun (x : tval) => #x) l) }}} insert_list (v, (#target))%V {{{ r, RET r; is_list r (map (fun (x : tval) => #x) (insert_list_spec target l)) }}}.
     Proof.
       clear bpos.
       iIntros (Φ) "Hl HPost".
@@ -149,7 +156,7 @@ Section bplus_tree.
             iIntros (?) "Hr".
             wp_store; wp_pure.
             iApply "HPost".
-            unfold Insert_list.
+            unfold insert_list_spec.
             rewrite (bool_decide_false_Zeqb _ _ Heqb0).
             rewrite bool_decide_eq_true in Heqb1;
               apply Z.ltb_lt in Heqb1;
@@ -159,7 +166,7 @@ Section bplus_tree.
             done.
           * wp_alloc new as "Hnew"; wp_pure.
             iApply "HPost".
-            unfold Insert_list;
+            unfold insert_list_spec;
               specialize (bool_decide_false_Zeqb _ _ Heqb0) as ?;
               rewrite bool_decide_eq_false in Heqb1;
               assert (Z.le target x) by lia;
@@ -177,27 +184,343 @@ Section bplus_tree.
             done.
     Qed.
 
-    Lemma insert_nary_tree_spec (t : nary_tree) (t_wf : nary_tree_wf_no_len b t) (v : val) (target : tval) :
-      {{{ is_node v t }}} insert_bplus_tree (v, #target)%V {{{ r, RET r; is_node r (Insert_nary_tree target t) }}}.
+    Lemma length_list_spec_proof (v : val) (l : list val):
+      {{{ is_list v l }}} length_list v {{{ r, RET #r; ⌜r = Z.of_nat (length l)⌝ ∗ is_list v l }}}.
+    Proof.
+      iIntros (Φ) "Hl HPost".
+
+      iInduction l as [] "IH" forall (Φ v).
+      - iDestruct "Hl" as "->".
+        wp_rec; wp_pures.
+        iApply ("HPost" $! 0).
+        done.
+      - iDestruct "Hl" as (l' ?) "(-> & Hl' & Hl)".
+        wp_rec; wp_load; wp_pure; wp_bind (length_list _).
+        iApply ("IH" with "[Hl]"); [iFrame|].
+        iNext.
+        iIntros (?) "[-> Hl]".
+        wp_pure.
+        iApply ("HPost" $! (1 + length l)%Z).
+        iSplitR;
+          [ iPureIntro; rewrite Z.add_1_l Nat2Z.inj_succ; done
+          | iExists l', hd'; iFrame; done ].
+    Qed.
+
+    Lemma firstn_nil {A} n : @firstn A n [] = [].
+    Proof. induction n; done. Qed.
+
+    Lemma skipn_nil {A} n : @skipn A n [] = [].
+    Proof. induction n; done. Qed.
+
+    Lemma split_list_spec_proof (v : val) (l : list val) (n : nat):
+      {{{ is_list v l }}} split_list (v, #(Z.of_nat n))%V {{{ r, RET (r.1, r.2); is_list r.1 (firstn n l) ∗ is_list r.2 (skipn n l) }}}.
+    Proof.
+      clear bpos.
+      iIntros (Φ) "Hl HPost".
+      iInduction n as [] "IH" forall (Φ v l).
+      - wp_rec; wp_pures.
+        iApply ("HPost" $! (InjLV #(), v)).
+        unfold take, drop.
+        cbn.
+        iFrame.
+        done.
+      - wp_rec; wp_pures;
+          destruct l.
+        + iDestruct "Hl" as "->".
+          wp_pures.
+          iApply ("HPost" $! (InjLV #(), InjLV #())).
+          rewrite firstn_nil skipn_nil.
+          done.
+
+        + iDestruct "Hl" as (l' ?) "(-> & Hl' & Hl)".
+          wp_load; wp_load; wp_pures; wp_bind (split_list _).
+          replace (Z.sub (S n) 1) with (Z.of_nat n) by lia.
+          iApply ("IH" with "[Hl]"); [done|].
+          iNext.
+          iIntros (?) "[Hr1 Hr2]".
+          wp_store; wp_pures.
+          iApply ("HPost" $! (InjRV #l', r.2)).
+          iSplitL "Hl' Hr1"; [iExists l', r.1; iFrame; done|].
+          done.
+    Qed.
+
+  Fixpoint insert_nary_tree_spec (target : Z) (t : nary_tree) : nary_tree * option nary_tree :=
+    match t with
+    | leaf (low, high) vals =>
+        let new_vals := insert_list_spec target vals in
+        if Z.ltb b (length new_vals)
+        then
+          let left_vals := firstn (b/2) new_vals in
+          let right_vals := skipn (b/2) new_vals in
+          let left_interval := (low, List.last left_vals high) in
+          let right_interval := (hd low right_vals, high) in
+          (* TODO: fix interval *)
+          (leaf (low, high) left_vals, Some (leaf (low, high) right_vals))
+        else
+          (leaf (low, high) new_vals, None)
+    | node (low, high) branches =>
+        let new_branches :=
+          ((fix insert_aux (l : list nary_tree) :=
+              match l with
+              | [] => []
+              | t :: [] =>
+                  let (new_t1, new_t2) := insert_nary_tree_spec target t in
+                  match new_t2 with
+                  | None => [new_t1]
+                  | Some new_t2' => new_t1 :: [new_t2']
+                  end
+              | t :: ts =>
+                  let (low, high) := (match t with leaf interval _ | node interval _ => interval end) in
+                  if andb (Z.leb low target) (Z.leb target high)
+                  then let (new_t1, new_t2) := insert_nary_tree_spec target t in
+                       match new_t2 with
+                       | None => new_t1 :: ts
+                       | Some new_t2' => new_t1 :: new_t2' :: ts
+                       end
+                  else t :: insert_aux ts
+              end) branches) in
+        if Z.ltb b (length new_branches)
+        then
+          let left_branches := firstn (b/2) new_branches in
+          let right_branches := skipn (b/2) new_branches in
+          let left_interval := (low, (List.last (map snd (map nary_tree_interval left_branches)) high)) in
+          let right_interval := (hd low (map fst (map nary_tree_interval right_branches)), high) in
+          (* TODO: should change intervals *)
+          (node (low, high) left_branches, Some (node (low, high) right_branches))
+        else
+          (node (low, high) new_branches, None)
+    end.
+
+    Definition insert_nary_tree : val :=
+      rec: "insert_nary_tree" "arg" :=
+        let: "t" := Fst "arg" in
+        let: "target" := Snd "arg" in
+        match: "t" with
+          InjL "ptr" =>
+            let: "lhd" := Snd !"ptr" in
+            let: "new" := insert_list ("lhd", "target") in
+            (* TODO: should change interval here *)
+            if: #b < length_list "new"
+            then
+              let: "newlpair" := split_list ("new", #(b/2)) in
+              let: "newleaf" := ref (Fst !"ptr", Snd "newlpair") in
+              "ptr" <- (Fst !"ptr", Fst "newlpair") ;;
+              (token_leaf_e "ptr", SOME (token_leaf_e "newleaf"))
+            else
+              "ptr" <- (Fst !"ptr", "new") ;;
+              (token_leaf_e "ptr", NONEV)
+        | InjR "ptr" =>
+            let: "lhd" := Snd !"ptr" in
+            let: "new" :=
+              (rec: "insert_node_list" "arg" :=
+                 let: "p" := Fst "arg" in
+                 let: "target" := Snd "arg" in
+                 match: "p" with
+                   NONE =>
+                     NONE
+                 | SOME "l" =>
+                     match: Snd !"l" with
+                       NONE =>
+                         let: "newt" := "insert_nary_tree" (Fst !"l", "target") in
+                         match: Snd "newt" with
+                           NONE => "l" <- (Fst "newt", NONE)
+                         | SOME "newt2" =>
+                             let: "l'" := ref ("newt2", NONE) in
+                             "l" <- (Fst "newt", SOME "l'")
+                         end
+                     | SOME "_" =>
+                         let: "thd" := Fst !"l" in
+                         let: "interval" :=
+                           match: "thd" with
+                             InjL "ptr" => Fst !"ptr"
+                           | InjR "ptr" => Fst !"ptr"
+                           end in
+                         let: "low" := Fst "interval" in
+                         let: "high" := Snd "interval" in
+                         (if: (BinOp LeOp "low" "target") && (BinOp LeOp "target" "high")
+                          then let: "newt" := "insert_nary_tree" ("thd", "target") in
+                               (* TODO: should change interval here *)
+                               match: Snd "newt" with
+                                 NONE => "l" <- (Fst "newt", Snd !"l")
+                               | SOME "newt2" =>
+                                   let: "l'" := ref ("newt2", Snd !"l") in
+                                   "l" <- (Fst "newt", SOME "l'")
+                               end
+                          else let: "newl" := "insert_node_list" (Snd !"l", "target") in
+                               "l" <- ("thd", "newl"))
+                     end ;; SOME "l"
+                 end) ("lhd", "target") in
+            if: #b < length_list "new"
+            then
+              let: "newlpair" := split_list ("new", #(b/2)) in
+              let: "newbranch" := ref (Fst !"ptr", Snd "newlpair") in
+              "ptr" <- (Fst !"ptr", Fst "newlpair") ;;
+              (token_branch_e "ptr", SOME (token_branch_e "newbranch"))
+            else
+              "ptr" <- (Fst !"ptr", "new") ;;
+              (token_branch_e "ptr", NONEV)
+        end%E.
+
+    Lemma branch_node_list_lengths : forall ns ts,
+      (fix branch_node_list (ns0 : list val) (ts0 : list nary_tree) {struct ts0} : iProp :=
+         match ns0 with
+         | [] => match ts0 with
+                | [] => True
+                | _ :: _ => False
+                end
+         | n :: ns1 =>
+             match ts0 with
+             | [] => False
+             | t :: ts1 => is_node n t ∗ branch_node_list ns1 ts1
+             end
+         end) ns ts -∗
+        (fix branch_node_list (ns0 : list val) (ts0 : list nary_tree) {struct ts0} : iProp :=
+         match ns0 with
+         | [] => match ts0 with
+                | [] => True
+                | _ :: _ => False
+                end
+         | n :: ns1 =>
+             match ts0 with
+             | [] => False
+             | t :: ts1 => is_node n t ∗ branch_node_list ns1 ts1
+             end
+         end) ns ts ∗ ⌜length ns = length ts⌝.
+    Proof.
+      iIntros (? ?).
+      iInduction ts as [|thd trest] "IH'" forall (ns);
+        destruct ns as [|nhd nrest]; [done|done|done|].
+      iIntros "[Hnhd Hnrest]".
+      iDestruct ("IH'" with "Hnrest") as "[Hnrest %]".
+      iSplitL; [iFrame|].
+      cbn.
+      rewrite H.
+      done.
+    Qed.
+
+    Lemma branch_node_split ns ts n :
+      (fix branch_node_list (ns1 : list val) (ts0 : list nary_tree) {struct ts0} : iProp :=
+         match ns1 with
+         | [] => match ts0 with
+                | [] => True
+                | _ :: _ => False
+                end
+         | n :: ns2 =>
+             match ts0 with
+             | [] => False
+             | t :: ts1 => is_node n t ∗ branch_node_list ns2 ts1
+             end
+         end) ns ts -∗
+        (fix branch_node_list (ns1 : list val) (ts0 : list nary_tree) {struct ts0} : iProp :=
+           match ns1 with
+           | [] => match ts0 with
+                  | [] => True
+                  | _ :: _ => False
+                  end
+           | n :: ns2 =>
+               match ts0 with
+               | [] => False
+               | t :: ts1 => is_node n t ∗ branch_node_list ns2 ts1
+               end
+           end) (take n ns) (take n ts) ∗
+        (fix branch_node_list (ns1 : list val) (ts0 : list nary_tree) {struct ts0} : iProp :=
+           match ns1 with
+           | [] => match ts0 with
+                  | [] => True
+                  | _ :: _ => False
+                  end
+           | n :: ns2 =>
+               match ts0 with
+               | [] => False
+               | t :: ts1 => is_node n t ∗ branch_node_list ns2 ts1
+               end
+           end) (drop n ns) (drop n ts).
+    Proof.
+      iIntros "Hns".
+      iInduction n as [] "IH" forall (ts ns); [repeat rewrite take_0; repeat rewrite drop_0; iFrame|].
+      destruct ns as [|nhd nrest]; destruct ts as [|thd trest]; [repeat rewrite take_nil;done|done|done|].
+      cbn; fold (@take val) (@take nary_tree) (@drop val) (@drop nary_tree).
+      iDestruct "Hns" as "[Hnhd Hnrest]".
+      iFrame.
+      iApply "IH"; done.
+    Qed.
+
+    Lemma insert_nary_tree_spec_proof (t : nary_tree) (t_wf : nary_tree_wf_no_len b t) (v : val) (target : tval) :
+      {{{ is_node v t }}}
+        insert_nary_tree (v, #target)%V
+        {{{ r, RET (r.1, r.2);
+            is_node r.1 (insert_nary_tree_spec target t).1 ∗
+              ((∃ (t2 : nary_tree),
+                   ⌜(insert_nary_tree_spec target t).2 = Some t2⌝ ∗
+                     ∃ (r2 : val), ⌜r.2 = SOMEV r2⌝ ∗ is_node r2 t2) ∨
+                 (⌜(insert_nary_tree_spec target t).2 = None⌝ ∗ ⌜r.2 = NONEV⌝))
+        }}}.
     Proof using bpos.
       iIntros (Φ) "Hv HPost".
 
       iInduction t as [(low & high)|(low & high) ts] "IH" using nary_tree_ind' forall (Φ v).
       - iPoseProof (tree_leaf_token_leaf with "Hv") as (?) "->".
         iDestruct "Hv" as (? ?) "(% & Hptr & Hlhd)".
-        assert (x = #ptr) by (unfold token_leaf_v in H; congruence); subst.
+        assert (x = #ptr) by (unfold token_leaf_v in H; congruence); subst; clear H.
         wp_rec; wp_load; wp_pures; wp_bind (insert_list _).
-        iApply (insert_list_spec with "Hlhd").
+        iApply (insert_list_spec_proof with "Hlhd").
         iNext.
         iIntros (?) "Hr".
-        wp_load; wp_store.
-        iApply "HPost".
-        iExists ptr, r.
-        iFrame.
-        done.
+        wp_pures; wp_bind (length_list _).
+        iApply (length_list_spec_proof with "Hr").
+        iNext.
+        iIntros (?) "[% Hr]".
+        wp_pure.
+        destruct (bool_decide (Z.lt b r0)) eqn:?.
+        + wp_pure; wp_bind (split_list _); wp_pure.
+          replace (Z.div b 2) with (Z.of_nat (b `div` 2)); [|admit]. (* TODO: just annoying arithmetic *)
+          iApply (split_list_spec_proof with "Hr").
+          iNext.
+          iIntros (?) "[Hr1 Hr2]".
+          wp_load; wp_alloc ptr' as "Hptr'"; wp_load; wp_store; wp_pures.
+          iApply ("HPost" $! (InjLV #ptr, InjRV (InjLV #ptr'))).
+          rewrite map_length in H; subst r0.
+          rewrite bool_decide_eq_true in Heqb0;
+            apply Z.ltb_lt in Heqb0.
+          iSplitL "Hptr Hr1".
+          { cbn; rewrite Heqb0.
+            iExists ptr, r1.1.
+            iSplitR; [done|].
+            iSplitL "Hptr"; [done|].
+            rewrite firstn_map; done. }
+          iLeft.
+          iExists (leaf (low, high) (drop (b `div` 2) (insert_list_spec target vals))).
+          iSplitR. { cbn; rewrite Heqb0; cbn; done. }
+          iExists (InjLV #ptr').
+          iSplitR; [done|].
+          iExists ptr', r1.2.
+          rewrite skipn_map.
+          iFrame.
+          done.
+
+        + wp_load; wp_store; wp_pures.
+          iApply ("HPost" $! (token_leaf_v #ptr, NONEV)).
+          apply bool_decide_eq_false_1 in Heqb0;
+              assert (Z.le r0 b) by lia;
+              apply Z.leb_le in H0;
+              rewrite Z.leb_antisym in H0;
+              symmetry in H0;
+              apply negb_sym in H0;
+              cbn in H0.
+          rewrite map_length in H; subst r0.
+          iSplitL.
+          { unfold insert_nary_tree_spec.
+            rewrite H0.
+            iExists ptr, r.
+            iFrame.
+            done. }
+          iRight.
+          cbn.
+          rewrite H0.
+          done.
+
       - iPoseProof (tree_node_token_branch with "Hv") as (?) "->".
-        iDestruct "Hv" as (ptr lhd ns) "(% & Hptr & Hlhd & Hns)".
-        fold is_node.
+        iDestruct "Hv" as (ptr lhd ns) "(% & Hptr & Hlhd & Hns)"; fold is_node.
         assert (x = #ptr) by (unfold token_branch_v in H; congruence); subst.
         wp_rec; wp_load; wp_proj; wp_let; wp_pure; wp_pure.
         iEval (cbn) in "HPost".
@@ -219,241 +542,283 @@ Section bplus_tree.
                        end
                    end) ns ts -∗
                 (∀ r : val,
-                    (∃ (ns0 : list val),
-                        is_list r ns0 ∗
-                          (fix branch_node_list (ns1 : list val) (ts0 : list nary_tree) {struct ts0} : iProp :=
-                             match ns1 with
+                    (∃ ns,
+                        is_list r ns ∗
+                          (fix branch_node_list (ns0 : list val) (ts0 : list nary_tree) {struct ts0} : iProp :=
+                             match ns0 with
                              | [] => match ts0 with
                                     | [] => True
                                     | _ :: _ => False
                                     end
-                             | n :: ns2 =>
+                             | n :: ns1 =>
                                  match ts0 with
                                  | [] => False
-                                 | t :: ts1 => is_node n t ∗ branch_node_list ns2 ts1
+                                 | t :: ts1 => is_node n t ∗ branch_node_list ns1 ts1
                                  end
-                             end) ns0
-                          ((fix insert_aux (l0 : list nary_tree) : list nary_tree :=
-                              match l0 with
-                              | [] => [leaf (target, target)%Z [target]]
-                              | t :: ts0 =>
+                             end) ns
+                          ((fix insert_aux (l : list nary_tree) : list nary_tree :=
+                              match l with
+                              | [] => []
+                              | [t] =>
+                                  let (new_t1, new_t2) := insert_nary_tree_spec target t in
+                                  match new_t2 with
+                                  | Some new_t2' => [new_t1; new_t2']
+                                  | None => [new_t1]
+                                  end
+                              | t :: (_ :: _) as ts0 =>
                                   let (low0, high0) :=
                                     match t with
                                     | leaf interval _ | node interval _ => interval
                                     end in
                                   if (low0 <=? target)%Z && (target <=? high0)%Z
-                                  then Insert_nary_tree target t :: ts0
+                                  then
+                                    let (new_t1, new_t2) := insert_nary_tree_spec target t in
+                                    match new_t2 with
+                                    | Some new_t2' => new_t1 :: new_t2' :: ts0
+                                    | None => new_t1 :: ts0
+                                    end
                                   else t :: insert_aux ts0
                               end) ts)) -∗ Φ' r) -∗
                 WP (rec: "insert_node_list" "arg" :=
-                      let: "p" := Fst "arg" in
-                      let: "target" := Snd "arg" in
-                      match: "p" with
-                        NONE =>
-                          let: "l" := SOME (ref ("target", NONE)) in
-                          let: "t" := ref (("target", "target"), "l") in
-                          SOME (ref (token_leaf_e "t", NONE))
-                      | SOME "l" =>
-                          let: "thd" := Fst !"l" in
-                          let: "interval" :=
-                            match: "thd" with
-                              InjL "ptr" => Fst !"ptr"
-                            | InjR "ptr" => Fst !"ptr"
-                            end in
-                          let: "low" := Fst "interval" in
-                          let: "high" := Snd "interval" in
-                          (if: (BinOp LeOp "low" "target") && (BinOp LeOp "target" "high")
-                           then let: "newt" := insert_bplus_tree ("thd", "target") in
-                                (* should change interval here *)
-                                "l" <- ("newt", Snd !"l")
-                           else let: "newl" := "insert_node_list" (Snd !"l", "target") in
-                                "l" <- ("thd", "newl")) ;;
-                          SOME "l"
-                      end)%V (lhd, #target)%V
+                 let: "p" := Fst "arg" in
+                 let: "target" := Snd "arg" in
+                 match: "p" with
+                   NONE =>
+                     NONE
+                 | SOME "l" =>
+                     match: Snd !"l" with
+                       NONE =>
+                         let: "newt" := insert_nary_tree (Fst !"l", "target") in
+                         match: Snd "newt" with
+                           NONE => "l" <- (Fst "newt", NONE)
+                         | SOME "newt2" =>
+                             let: "l'" := ref ("newt2", NONE) in
+                             "l" <- (Fst "newt", SOME "l'")
+                         end
+                     | SOME "_" =>
+                         let: "thd" := Fst !"l" in
+                         let: "interval" :=
+                           match: "thd" with
+                             InjL "ptr" => Fst !"ptr"
+                           | InjR "ptr" => Fst !"ptr"
+                           end in
+                         let: "low" := Fst "interval" in
+                         let: "high" := Snd "interval" in
+                         (if: (BinOp LeOp "low" "target") && (BinOp LeOp "target" "high")
+                          then let: "newt" := insert_nary_tree ("thd", "target") in
+                               (* TODO: should change interval here *)
+                               match: Snd "newt" with
+                                 NONE => "l" <- (Fst "newt", Snd !"l")
+                               | SOME "newt2" =>
+                                   let: "l'" := ref ("newt2", Snd !"l") in
+                                   "l" <- (Fst "newt", SOME "l'")
+                               end
+                          else let: "newl" := "insert_node_list" (Snd !"l", "target") in
+                               "l" <- ("thd", "newl"))
+                     end ;; SOME "l"
+                 end)%V (lhd, #target)%V
                 {{ v, Φ' v}}
           )%I as "IH'".
         { iIntros (Φ') "[Hlhd Hns] HPost".
           inversion_clear t_wf
-            as [| ? ? ? ? _ _ trees_wf _].
+            as [| ? ? ? ? _ _ trees_wf _];
             subst intervals.
 
           iInduction ts as [|thd trest] "IH'" forall (Φ' ns lhd);
             destruct ns as [|nhd nrest]; [|done|done|].
           - iDestruct "Hlhd" as "->".
-
-            wp_alloc newl as "Hnewl";
-              wp_alloc newt as "Hnewt";
-              wp_alloc newts as "Hnewts";
-              wp_pure.
+            wp_pures.
             iApply "HPost".
-            iExists [ token_leaf_v #newt ].
-            iFrame.
-            iSplitL "Hnewts"; [iExists newts, (InjLV #()); iFrame; done|].
-            iExists newt, (InjRV #newl).
-            iFrame.
-            iSplitR; [done|].
-            iExists newl, (InjLV #()).
-            iFrame.
+            iExists [].
             done.
-          - iEval (rewrite big_opL_cons) in "IH".
-            iDestruct "IH" as "[IHthd IHtrest]".
-            apply Forall_cons in trees_wf.
-            destruct trees_wf as [thd_wf trest_wf].
 
-            iDestruct "Hlhd" as (l0 ?) "(-> & Hl0 & Hnrest)".
-            destruct thd.
-            * destruct interval as [low' high'].
-              iDestruct "Hns" as "[Hthd Hns]".
-              iDestruct "Hthd" as (ptr' leaves) "(-> & Hptr' & Hleaves)".
+          - iDestruct "Hns" as "[Hnhd Hnrest]".
+            destruct trest as [|tsnd]; destruct nrest as [|nsnd]; [|done|done|];
+              iEval (rewrite big_opL_cons) in "IH";
+              iDestruct "IH" as "[IHthd IHtrest]";
+              apply Forall_cons in trees_wf;
+              destruct trees_wf as [thd_wf trest_wf];
+              apply nary_tree_wf_remove_len in thd_wf.
+            + iDestruct "Hlhd" as (l0 ?) "(-> & Hl0 & ->)".
+              wp_load; wp_load; wp_pures; wp_bind (insert_nary_tree _).
+              iApply ("IHthd" $! thd_wf with "Hnhd").
+              iNext.
+              iIntros (?) "[Hr1 Hr2]".
+              iDestruct "Hr2" as "[(% & % & % & -> & Hr2) | (% & ->)]";
+                destruct (insert_nary_tree_spec target thd) as [new_t1 new_t2];
+                cbn in H0; subst.
+              * wp_alloc lr2 as "Hlr2"; wp_store; wp_pure.
+                iApply "HPost".
+                iExists (r.1 :: r2 :: []).
+                iSplitL "Hl0 Hlr2";
+                  [iExists l0, (SOMEV #lr2); iFrame; iSplitR; [done|]; iExists lr2, NONEV; iFrame; done|].
+                iFrame; done.
+              * wp_store; wp_pure.
+                iApply "HPost".
+                iExists [r.1].
+                iSplitL "Hl0"; [iExists l0, NONEV; iFrame; done|].
+                iFrame; done.
+
+            + iDestruct "Hlhd" as (l1 ?) "(-> & Hl1 & Hhd')".
+              iDestruct "Hhd'" as (l2 ?) "(-> & Hl2 & Hhd')".
               wp_load; wp_load; wp_pures.
-              destruct (bool_decide (Z.le low' target)) eqn:?; wp_pures.
-              -- destruct (bool_decide (Z.le target high')) eqn:?; wp_pures.
-                 ++ wp_bind (insert_bplus_tree _).
-                    iApply ("IHthd" with "[] [Hptr' Hleaves]").
-                    { apply nary_tree_wf_remove_len in thd_wf; done. }
-                    { iExists ptr', leaves; iFrame; done. }
-                    iNext.
-                    iIntros (?) "Hr".
-                    wp_load; wp_store; wp_pure.
-                    iApply "HPost".
-                    iExists (r :: nrest).
-                    iSplitL "Hl0 Hnrest".
-                    { iExists l0, hd'; iFrame; done. }
-                    apply bool_decide_eq_true_1 in Heqb0;
-                      apply Z.leb_le in Heqb0;
-                      rewrite Heqb0.
-                    apply bool_decide_eq_true_1 in Heqb1;
-                      apply Z.leb_le in Heqb1;
-                      rewrite Heqb1.
-                    iFrame.
-                    done.
+              destruct thd.
+              * destruct interval as [low' high'].
+                iDestruct "Hnhd" as (ptr' leaves) "(-> & Hptr' & Hleaves)".
+                wp_load; wp_pures.
+                destruct (bool_decide (Z.le low' target)) eqn:?; wp_pures.
+                -- destruct (bool_decide (Z.le target high')) eqn:?; wp_pures.
+                   ++ wp_bind (insert_nary_tree _).
+                      iApply ("IHthd" $! thd_wf with "[Hptr' Hleaves]").
+                      { iExists ptr', leaves; iFrame; done. }
+                      iNext.
+                      iIntros (?) "[Hr1 Hr2]".
+                      apply bool_decide_eq_true_1 in Heqb0;
+                           apply Z.leb_le in Heqb0;
+                           rewrite Heqb0.
+                         apply bool_decide_eq_true_1 in Heqb1;
+                           apply Z.leb_le in Heqb1;
+                           rewrite Heqb1.
+                      iDestruct "Hr2" as "[(% & % & % & -> & Hr2) | (% & ->)]";
+                        destruct (insert_nary_tree_spec target (leaf (low', high') l)) as [new_t1 new_t2];
+                        cbn in H0; subst.
+                      ** wp_load; wp_alloc l3 as "Hl3"; wp_store; wp_pure.
+                         iApply "HPost".
+                         iExists (r.1 :: r2 :: nsnd :: nrest).
+                         iSplitL "Hl1 Hl3 Hl2 Hhd'";
+                           [iExists l1, (SOMEV #l3); iFrame; iSplitR; [done|]; iExists l3, (SOMEV #l2); iFrame; iSplitR; [done|]; iExists l2, hd'0; iFrame; done|].
+                         iFrame; done.
+                      ** wp_load; wp_store; wp_pure.
+                         iApply "HPost".
+                         iExists (r.1 :: nsnd :: nrest).
+                         iSplitL "Hl1 Hl2 Hhd'";
+                           [iExists l1, (SOMEV #l2); iFrame; iSplitR; [done|]; iExists l2, hd'0; iFrame; done|].
+                         iFrame; done.
+                   ++ wp_load; wp_pure; wp_pure.
+                      wp_bind ((rec: "insert_node_list" "arg" := _) (SOMEV #l2, #target))%V.
+                      iApply ("IH'" $! trest_wf _ (nsnd :: nrest) (SOMEV #l2) with "[] [Hl2 Hhd'] [Hnrest]"); try done.
+                      { iExists l2, hd'0; iFrame; done. }
+                      iIntros (?) "[% [Hr Hns]]".
+                      wp_store; wp_pure.
+                      iApply "HPost".
+                      apply bool_decide_eq_true_1 in Heqb0;
+                        apply Z.leb_le in Heqb0;
+                        rewrite Heqb0.
+                      apply bool_decide_eq_false_1 in Heqb1;
+                        assert (Z.lt high' target) by lia;
+                        apply Z.ltb_lt in H0;
+                        rewrite Z.ltb_antisym in H0;
+                        symmetry in H0;
+                        apply negb_sym in H0;
+                        cbn in H0;
+                        rewrite H0.
+                      iExists (token_leaf_v #ptr' :: ns).
+                      iFrame.
+                      iSplitL "Hl1 Hr"; [iExists l1, r; iFrame; done|].
+                      iExists ptr', leaves; iFrame; done.
+                -- wp_load; wp_pure; wp_pure;
+                     wp_bind ((rec: "insert_node_list" "arg" := _) (SOMEV #l2, #target))%V.
+                   iApply ("IH'" $! trest_wf _ (nsnd :: nrest) with "[] [Hl2 Hhd'] [Hnrest]"); try done.
+                   { iExists l2, hd'0; iFrame; done. }
+                   iIntros (?) "[% [Hr Hns]]".
+                   wp_store; wp_pures.
+                   iApply "HPost".
 
-                 ++ wp_load; wp_pure; wp_pure;
-                      wp_bind ((rec: "insert_node_list" "arg" := _) (hd', #target))%V.
-                    iApply ("IH'" with "[] [] [Hnrest] [Hns]"); try done.
-                    iIntros (?) "[% [Hr Hns0]]".
-                    wp_store; wp_pure.
-                    iApply "HPost".
-                    apply bool_decide_eq_true_1 in Heqb0;
-                      apply Z.leb_le in Heqb0;
-                      rewrite Heqb0.
-                    apply bool_decide_eq_false_1 in Heqb1;
-                      assert (Z.lt high' target) by lia;
-                      apply Z.ltb_lt in H0;
-                      rewrite Z.ltb_antisym in H0;
-                      symmetry in H0;
-                      apply negb_sym in H0;
-                      cbn in H0;
-                      rewrite H0.
-                    cbn.
-                    iExists (token_leaf_v #ptr' :: ns0).
-                    iFrame.
-                    iSplitL "Hl0 Hr".
-                    { iExists l0, r; iFrame; done. }
-                    iExists ptr', leaves; iFrame; done.
+                   apply bool_decide_eq_false_1 in Heqb0;
+                     assert (Z.lt target low') by lia;
+                     apply Z.ltb_lt in H0;
+                     rewrite Z.ltb_antisym in H0;
+                     symmetry in H0;
+                     apply negb_sym in H0;
+                     cbn in H0;
+                     rewrite H0.
+                   iExists (token_leaf_v #ptr' :: ns).
+                   iFrame.
+                   iSplitL "Hl1 Hr"; [iExists l1, r; iFrame; done|].
+                   iExists ptr', leaves; iFrame; done.
 
-              -- wp_load; wp_pure; wp_pure;
-                   wp_bind ((rec: "insert_node_list" "arg" := _) (hd', #target))%V.
-                 iApply ("IH'" with "[] [] [Hnrest] [Hns]"); try done.
-                 iIntros (?) "[% [Hr Hns0]]".
-                 wp_store; wp_pures.
-                 iApply "HPost".
+              * admit. (* TODO: repeat for node (or find a better way to get interval out) *) }
 
-                 apply bool_decide_eq_false_1 in Heqb0;
-                   assert (Z.lt target low') by lia;
-                   apply Z.ltb_lt in H0;
-                   rewrite Z.ltb_antisym in H0;
-                   symmetry in H0;
-                   apply negb_sym in H0;
-                   cbn in H0;
-                   rewrite H0.
-                 iExists (token_leaf_v #ptr' :: ns0).
-                 iFrame.
-                 iSplitL "Hl0 Hr".
-                 { iExists l0, r; iFrame; done. }
-                 iExists ptr', leaves; iFrame; done.
-
-            * destruct interval as [low' high'].
-              iDestruct "Hns" as "[Hthd Hns]".
-              iDestruct "Hthd" as (ptr' leaves) "(% & -> & Hptr' & Hleaves)".
-              wp_load; wp_load; wp_pures.
-              destruct (bool_decide (Z.le low' target)) eqn:?; wp_pures.
-              -- destruct (bool_decide (Z.le target high')) eqn:?; wp_pures.
-                 ++ wp_bind (insert_bplus_tree _).
-                    iApply ("IHthd" with "[] [Hptr' Hleaves]").
-                    { apply nary_tree_wf_remove_len in thd_wf; done. }
-                    { iExists ptr', leaves, ns; iFrame; done. }
-                    iNext.
-                    iIntros (?) "Hr".
-                    wp_load; wp_store; wp_pure.
-                    iApply "HPost".
-                    iExists (r :: nrest).
-                    iSplitL "Hl0 Hnrest".
-                    { iExists l0, hd'; iFrame; done. }
-                    apply bool_decide_eq_true_1 in Heqb0;
-                      apply Z.leb_le in Heqb0;
-                      rewrite Heqb0.
-                    apply bool_decide_eq_true_1 in Heqb1;
-                      apply Z.leb_le in Heqb1;
-                      rewrite Heqb1.
-                    iFrame.
-                    done.
-
-                 ++ wp_load; wp_pure; wp_pure;
-                      wp_bind ((rec: "insert_node_list" "arg" := _) (hd', #target))%V.
-                    iApply ("IH'" with "[] [] [Hnrest] [Hns]"); try done.
-                    iIntros (?) "[% [Hr Hns0]]".
-                    wp_store; wp_pure.
-                    iApply "HPost".
-                    apply bool_decide_eq_true_1 in Heqb0;
-                      apply Z.leb_le in Heqb0;
-                      rewrite Heqb0.
-                    apply bool_decide_eq_false_1 in Heqb1;
-                      assert (Z.lt high' target) by lia;
-                      apply Z.ltb_lt in H0;
-                      rewrite Z.ltb_antisym in H0;
-                      symmetry in H0;
-                      apply negb_sym in H0;
-                      cbn in H0;
-                      rewrite H0.
-                    iExists (token_branch_v #ptr' :: ns0).
-                    iFrame.
-                    iSplitL "Hl0 Hr".
-                    { iExists l0, r; iFrame; done. }
-                    iExists ptr', leaves, ns; iFrame; done.
-
-              -- wp_load; wp_pure; wp_pure;
-                   wp_bind ((rec: "insert_node_list" "arg" := _) (hd', #target))%V.
-                 iApply ("IH'" with "[] [] [Hnrest] [Hns]"); try done.
-                 iIntros (?) "[% [Hr Hns0]]".
-                 wp_store; wp_pures.
-                 iApply "HPost".
-
-                 apply bool_decide_eq_false_1 in Heqb0;
-                   assert (Z.lt target low') by lia;
-                   apply Z.ltb_lt in H0;
-                   rewrite Z.ltb_antisym in H0;
-                   symmetry in H0;
-                   apply negb_sym in H0;
-                   cbn in H0;
-                   rewrite H0.
-                 iExists (token_branch_v #ptr' :: ns0).
-                 iFrame.
-                 iSplitL "Hl0 Hr".
-                 { iExists l0, r; iFrame; done. }
-                 iExists ptr', leaves, ns; iFrame; done. }
-
-        iApply ("IH'" with "[Hlhd Hns]").
+        iClear "IH".
+        iApply ("IH'" with "[Hlhd Hns]"); iClear "IH'".
         { iFrame. }
-        
         iIntros (r) "Hr".
-        wp_load; wp_store; wp_pure.
-        iApply "HPost".
-        iDestruct "Hr" as (ns0) "[Hr Hns0]".
-        iExists ptr, r, ns0.
-        iFrame.
-        done.
-    Qed.
+        iDestruct "Hr" as (?) "[Hr Hns0]".
+
+        wp_pures; wp_bind (length_list _).
+        iApply (length_list_spec_proof with "Hr").
+        iNext.
+        iIntros (?) "[% Hr]".
+        wp_pure.
+        remember ((fix insert_aux (l : list nary_tree) : list nary_tree :=
+                     match l with
+                     | [] => []
+                     | [t] =>
+                         let (new_t1, new_t2) := insert_nary_tree_spec target t in
+                         match new_t2 with
+                         | Some new_t2' => [new_t1; new_t2']
+                         | None => [new_t1]
+                         end
+                     | t :: (_ :: _) as ts0 =>
+                         let (low0, high0) :=
+                           match t with
+                           | leaf interval _ | node interval _ => interval
+                           end in
+                         if (low0 <=? target)%Z && (target <=? high0)%Z
+                         then
+                           let (new_t1, new_t2) := insert_nary_tree_spec target t in
+                           match new_t2 with
+                           | Some new_t2' => new_t1 :: new_t2' :: ts0
+                           | None => new_t1 :: ts0
+                           end
+                         else t :: insert_aux ts0
+                     end) ts) as new_ts.
+        destruct (bool_decide (Z.lt b r0)) eqn:?.
+        + wp_pure; wp_bind (split_list _); wp_pure.
+          replace (Z.div b 2) with (Z.of_nat (b `div` 2)); [|admit]. (* TODO: just annoying arithmetic *)
+          iApply (split_list_spec_proof with "Hr").
+          iNext.
+          iIntros (?) "[Hr1 Hr2]".
+          wp_load; wp_alloc ptr' as "Hptr'"; wp_load; wp_store; wp_pures.
+          iApply ("HPost" $! (token_branch_v #ptr, token_branch_v (SOMEV #ptr'))).
+          subst r0.
+          rewrite bool_decide_eq_true in Heqb0;
+            apply Z.ltb_lt in Heqb0.
+          iPoseProof ((branch_node_list_lengths ns0 new_ts) with "Hns0") as "[Hns0 %Heqlengths]".
+          rewrite <- Heqlengths, Heqb0.
+          iPoseProof ((branch_node_split ns0 new_ts (b/2)) with "Hns0") as "[Htakens Hdropns]".
+
+          iSplitL "Hptr Hr1 Htakens".
+          { cbn.
+            iExists ptr, r1.1, (take (b/2) ns0).
+            iFrame.
+            done. }
+          iLeft.
+          iExists (node (low, high) (drop (b/2) new_ts)).
+          iSplitR; [done|].
+          iExists (token_branch_v #ptr').
+          iSplitR; [done|].
+          iExists ptr', r1.2, (drop (b/2) ns0).
+          iFrame.
+          done.
+
+        + wp_load; wp_store; wp_pures.
+          iApply ("HPost" $! (token_branch_v #ptr, NONEV)).
+          apply bool_decide_eq_false_1 in Heqb0;
+            assert (Z.le r0 b) by lia;
+            apply Z.leb_le in H1;
+            rewrite Z.leb_antisym in H1;
+            symmetry in H1;
+            apply negb_sym in H1;
+            cbn in H1.
+          subst r0.
+          iPoseProof ((branch_node_list_lengths ns0 new_ts) with "Hns0") as "[Hns0 %Heqlengths]".
+          rewrite <- Heqlengths, H1.
+
+          iSplitL "Hptr Hr Hns0"; [iExists ptr, r, ns0; iFrame; done|].
+          iRight.
+          done.
+    Admitted.
 
   End bplus_tree_proofs.
 End bplus_tree.
